proof/SimMemId.v
@@ -14,6 +14,7 @@ Require Import Integers.
 
 Require Import IntegersC LinkingC.
 Require Import SimDef SimSymb Skeleton Mod ModSem.
+Require SimSymbId.
 Require Import SimMem.
 
 Set Implicit Arguments.
@@ -70,127 +71,28 @@ Qed.
 
 
 
-Inductive sim_skenv (skenv0 skenv1: SkEnv.t): Prop :=
-| sim_skenv_intro
-    (NEXT: skenv0.(Genv.genv_next) = skenv1.(Genv.genv_next))
-    (SYMB: all1 (skenv0.(Genv.find_symbol) =1= skenv1.(Genv.find_symbol)))
-    (DEFS: all1 (skenv0.(Genv.find_def) =1= skenv1.(Genv.find_def)))
-    (PUBS: skenv0.(Genv.genv_public) = skenv1.(Genv.genv_public))
-.
-
-Goal sim_skenv = Genv.match_genvs eq.
-Proof.
-  apply Axioms.functional_extensionality; i.
-  apply Axioms.functional_extensionality; i.
-  apply AxiomsC.prop_ext.
-  split; i; inv H; econs; eauto.
-  - ii. unfold Genv.find_def in *. erewrite DEFS.
-    destruct ((Genv.genv_defs x0) ! b) eqn:T; econs; eauto.
-  - unfold Genv.find_def in *. i. specialize (mge_defs x1). inv mge_defs; ss.
-  - admit "".
-Qed.
-
-Inductive sim_sk (u: unit) (sk_src sk_tgt: Sk.t): Prop :=
-| sim_sk_intro
-    (SIM: match_program (fun _ => sim_fun) eq sk_src sk_tgt)
-.
-
 Global Program Instance SimSymbId: SimSymb.class SimMemId := {
   t := unit;
-  le := top4;
-  sim_sk := sim_sk;
-  sim_skenv (_: SimMem.t) (_: unit) := sim_skenv;
+  le := SimSymbId.le;
+  sim_sk := SimSymbId.sim_sk;
+  sim_skenv (_: SimMem.t) (_: unit) := SimSymbId.sim_skenv;
 }
 .
 Next Obligation.
-  inv SIMSK. inv SIMSK0.
-  SearchAbout TransfLink.
-  admit "this should hold".
+  ss.
 Qed.
 Next Obligation.
-  u in *. inv SIMSK.
-  Print Genv.init_mem_transf.
-  Print Genv.init_mem_transf_partial.
-  About Genv.init_mem_match.
-  exploit (Genv.init_mem_match SIM); eauto. i. clarify.
-  esplits; eauto.
-  - econs; eauto.
-    + erewrite ! Genv.init_mem_genv_next; eauto.
-    + i. symmetry. apply (Genv.find_symbol_match SIM).
-    + ii. hexploit (Genv.find_def_match_2 SIM x0); eauto. intro REL.
-      inv REL; ss. inv H2; ss.
-      * admit "remove sig then this will hold // or just now this will hold if we don't drop sig on opt".
-      * inv H3; ss.
-    + inv SIM; des; ss. rewrite ! Genv.globalenv_public. ss.
-  - instantiate (1:= mk _ _). ss.
-  - ss.
-  - ss.
-Unshelve.
+  eapply SimSymbId.sim_sk_link; eauto.
 Qed.
 Next Obligation.
-  inv LESRC.
-  inv LETGT.
-  inv SIMSKENV.
-  inv SIMSK. unfold match_program in *.
-  assert(DEFSEQ: sk_src.(defs) = sk_tgt.(defs)).
-  { apply Axioms.functional_extensionality. intro id.
-    hexploit (@match_program_defmap _ _ _ _ _ _ _ _ _ _ _ SIM).
-    instantiate (1:= id).
-    i.
-    inv H; ss.
-    - unfold defs.
-      admit "this is weak. add list_norept or prove my own theorem with induction.".
-    - admit "this will hold".
-  }
-  econs; eauto.
-  - eq_closure_tac.
-  - intro id.
-    destruct (Classical_Prop.classic (sk_src.(defs) id)); cycle 1.
-    + exploit SYMBDROP; eauto. i; des.
-      exploit SYMBDROP0; eauto. { rewrite <- DEFSEQ. eauto. } i; des.
-      rewrite H0. rewrite H1. ss.
-    + exploit SYMBKEEP; eauto. i; des.
-      exploit SYMBKEEP0; eauto. { rewrite <- DEFSEQ. eauto. } i; des.
-      rewrite H0. rewrite H1. ss.
-  - intro blk.
-    destruct (Genv.invert_symbol skenv_link_src blk) eqn:T0; cycle 1.
-    + rewrite DEFORPHAN; ss.
-      destruct (Genv.invert_symbol skenv_link_tgt blk) eqn:T1; cycle 1.
-      * rewrite DEFORPHAN0; ss.
-      * repeat all_once_fast ltac:(fun H => try apply Genv.invert_find_symbol in H; des).
-        rewrite <- SYMB in *.
-        repeat all_once_fast ltac:(fun H => try apply Genv.find_invert_symbol in H; des).
-        clarify.
-    + destruct (Genv.invert_symbol skenv_link_tgt blk) eqn:T1; cycle 1.
-      * repeat all_once_fast ltac:(fun H => try apply Genv.invert_find_symbol in H; des).
-        rewrite SYMB in *.
-        repeat all_once_fast ltac:(fun H => try apply Genv.find_invert_symbol in H; des).
-        clarify.
-      * repeat all_once_fast ltac:(fun H => try apply Genv.invert_find_symbol in H; des).
-        assert(i = i0).
-        { eapply Genv.genv_vars_inj; eauto. unfold Genv.find_symbol in *. rewrite SYMB. ss. }
-        clarify.
-        repeat all_once_fast ltac:(fun H => try apply Genv.find_invert_symbol in H; des).
-        destruct (classic (defs sk_src i0)).
-        { erewrite DEFKEEP; eauto. erewrite DEFKEEP0; eauto. rewrite <- DEFSEQ; ss. }
-        { erewrite DEFDROP; eauto. erewrite DEFDROP0; eauto. rewrite <- DEFSEQ; ss. }
-  - eq_closure_tac. ss. (* TODO: debug this *)
-    rewrite PUBLIC. rewrite PUBS. rewrite PUBLIC0. ss.
+  exploit SimSymbId.sim_sk_load_sim_skenv; eauto. i; des.
+  eexists. eexists (mk _ _).
+  esplits; ss; eauto.
 Qed.
 Next Obligation.
-  inv SIMSKENV.
-  econs; eauto.
-  - ii. ss.
-    assert(fptr_src = fptr_tgt).
-    { ss. }
-    clarify. unfold Genv.find_funct, Genv.find_funct_ptr in *. des_ifs_safe.
-    erewrite <- DEFS; eauto. des_ifs. esplits; eauto.
-    admit "just use eq".
-  - ii.
-    assert(fptr_src = fptr_tgt).
-    { ss. }
-    clarify. unfold Genv.find_funct, Genv.find_funct_ptr in *. des_ifs_safe.
-    erewrite DEFS; eauto. des_ifs. esplits; eauto.
-    admit "just use eq".
+  eapply SimSymbId.sim_skenv_monotone; try apply SIMSKENV; eauto.
+Qed.
+Next Obligation.
+  eapply SimSymbId.sim_skenv_func_bisim; eauto.
 Qed.
 
