proof/SimSymbId.v
@@ -1,0 +1,188 @@
+Require Import Events.
+Require Import Values.
+Require Import AST.
+Require Import Asmregs.
+Require Import Memory.
+Require Import Globalenvs.
+Require Import Smallstep.
+Require Import CoqlibC.
+Require Import Skeleton.
+Require Import Integers.
+Require Import ASTC.
+Require Import LinkingC.
+Require Import MapsC.
+
+
+Require Import SimDef SimSymb.
+
+
+Set Implicit Arguments.
+
+
+Inductive sim_skenv (skenv0 skenv1: SkEnv.t): Prop :=
+| sim_skenv_intro
+    (NEXT: skenv0.(Genv.genv_next) = skenv1.(Genv.genv_next))
+    (SYMB: all1 (skenv0.(Genv.find_symbol) =1= skenv1.(Genv.find_symbol)))
+    (DEFS: all1 (skenv0.(Genv.find_def) =1= skenv1.(Genv.find_def)))
+    (PUBS: skenv0.(Genv.genv_public) = skenv1.(Genv.genv_public))
+.
+
+Goal sim_skenv = Genv.match_genvs eq.
+Proof.
+  apply Axioms.functional_extensionality; i.
+  apply Axioms.functional_extensionality; i.
+  apply AxiomsC.prop_ext.
+  split; i; inv H; econs; eauto.
+  - ii. unfold Genv.find_def in *. erewrite DEFS.
+    destruct ((Genv.genv_defs x0) ! b) eqn:T; econs; eauto.
+  - unfold Genv.find_def in *. i. specialize (mge_defs x1). inv mge_defs; ss.
+  - admit "".
+Qed.
+
+Inductive sim_sk (u: unit) (sk_src sk_tgt: Sk.t): Prop :=
+| closed_intro
+    (SIM: match_program (fun _ => sim_fun) eq sk_src sk_tgt)
+.
+
+Definition le: unit -> Sk.t -> Sk.t -> unit -> Prop := top4.
+
+Lemma sim_sk_link: forall
+          ss0 (sk_src0 sk_tgt0: Sk.t)
+          (SIMSK: sim_sk ss0 sk_src0 sk_tgt0)
+          ss1 sk_src1 sk_tgt1
+          (SIMSK: sim_sk ss1 sk_src1 sk_tgt1)
+          sk_src
+          (LINKSRC: link sk_src0 sk_src1 = Some sk_src)
+        ,
+          exists ss sk_tgt,
+            <<LINKTGT: link sk_tgt0 sk_tgt1 = Some sk_tgt>> /\
+            <<LE0: le ss0 sk_src0 sk_tgt0 ss>> /\
+            <<LE1: le ss1 sk_src1 sk_tgt1 ss>> /\
+            <<SIMSK: sim_sk ss sk_src sk_tgt>>
+.
+Proof.
+  i.
+  inv SIMSK. inv SIMSK0.
+  SearchAbout TransfLink.
+  admit "this should hold".
+Qed.
+
+Lemma sim_sk_load_sim_skenv: forall
+          ss sk_src sk_tgt
+          (SIMSK: sim_sk ss sk_src sk_tgt)
+          skenv_src skenv_tgt
+          (LOADSRC: sk_src.(Sk.load_skenv) = skenv_src)
+          (LOADTGT: sk_tgt.(Sk.load_skenv) = skenv_tgt)
+          m_src
+          (LOADMEMSRC: sk_src.(Sk.load_mem) = Some m_src)
+        ,
+            (<<LOADMEMTGT: sk_tgt.(Sk.load_mem) = Some m_src>>) /\
+            (<<SIMSKENV: sim_skenv skenv_src skenv_tgt>>)
+.
+Proof.
+  i. u in *. inv SIMSK.
+  Print Genv.init_mem_transf.
+  Print Genv.init_mem_transf_partial.
+  About Genv.init_mem_match.
+  exploit (Genv.init_mem_match SIM); eauto. i. clarify.
+  esplits; eauto.
+  - econs; eauto.
+    + erewrite ! Genv.init_mem_genv_next; eauto.
+    + i. symmetry. apply (Genv.find_symbol_match SIM).
+    + ii. hexploit (Genv.find_def_match_2 SIM x0); eauto. intro REL.
+      inv REL; ss. inv H2; ss.
+      * admit "remove sig then this will hold // or just now this will hold if we don't drop sig on opt".
+      * inv H3; ss.
+    + inv SIM; des; ss. rewrite ! Genv.globalenv_public. ss.
+Qed.
+
+Lemma sim_skenv_monotone: forall
+          ss_link skenv_link_src skenv_link_tgt
+          (WFSRC: SkEnv.wf skenv_link_src)
+          (WFTGT: SkEnv.wf skenv_link_tgt)
+          (SIMSKENV: sim_skenv skenv_link_src skenv_link_tgt)
+          ss sk_src sk_tgt
+          (SIMSK: sim_sk ss sk_src sk_tgt)
+          (LE: le ss sk_src sk_tgt ss_link)
+          skenv_src skenv_tgt
+          (LESRC: SkEnv.project_spec skenv_link_src sk_src.(defs) skenv_src)
+          (LETGT: SkEnv.project_spec skenv_link_tgt sk_tgt.(defs) skenv_tgt)
+        ,
+          <<SIMSKENV: sim_skenv skenv_src skenv_tgt>>
+.
+Proof.
+  i.
+  inv LESRC.
+  inv LETGT.
+  inv SIMSKENV.
+  inv SIMSK. unfold match_program in *.
+  assert(DEFSEQ: sk_src.(defs) = sk_tgt.(defs)).
+  { apply Axioms.functional_extensionality. intro id.
+    hexploit (@match_program_defmap _ _ _ _ _ _ _ _ _ _ _ SIM).
+    instantiate (1:= id).
+    i.
+    inv H; ss.
+    - unfold defs.
+      admit "this is weak. add list_norept or prove my own theorem with induction.".
+    - admit "this will hold".
+  }
+  econs; eauto.
+  - eq_closure_tac.
+  - intro id.
+    destruct (Classical_Prop.classic (sk_src.(defs) id)); cycle 1.
+    + exploit SYMBDROP; eauto. i; des.
+      exploit SYMBDROP0; eauto. { rewrite <- DEFSEQ. eauto. } i; des.
+      rewrite H0. rewrite H1. ss.
+    + exploit SYMBKEEP; eauto. i; des.
+      exploit SYMBKEEP0; eauto. { rewrite <- DEFSEQ. eauto. } i; des.
+      rewrite H0. rewrite H1. ss.
+  - intro blk.
+    destruct (Genv.invert_symbol skenv_link_src blk) eqn:T0; cycle 1.
+    + rewrite DEFORPHAN; ss.
+      destruct (Genv.invert_symbol skenv_link_tgt blk) eqn:T1; cycle 1.
+      * rewrite DEFORPHAN0; ss.
+      * repeat all_once_fast ltac:(fun H => try apply Genv.invert_find_symbol in H; des).
+        rewrite <- SYMB in *.
+        repeat all_once_fast ltac:(fun H => try apply Genv.find_invert_symbol in H; des).
+        clarify.
+    + destruct (Genv.invert_symbol skenv_link_tgt blk) eqn:T1; cycle 1.
+      * repeat all_once_fast ltac:(fun H => try apply Genv.invert_find_symbol in H; des).
+        rewrite SYMB in *.
+        repeat all_once_fast ltac:(fun H => try apply Genv.find_invert_symbol in H; des).
+        clarify.
+      * repeat all_once_fast ltac:(fun H => try apply Genv.invert_find_symbol in H; des).
+        assert(i = i0).
+        { eapply Genv.genv_vars_inj; eauto. unfold Genv.find_symbol in *. rewrite SYMB. ss. }
+        clarify.
+        repeat all_once_fast ltac:(fun H => try apply Genv.find_invert_symbol in H; des).
+        destruct (classic (defs sk_src i0)).
+        { erewrite DEFKEEP; eauto. erewrite DEFKEEP0; eauto. rewrite <- DEFSEQ; ss. }
+        { erewrite DEFDROP; eauto. erewrite DEFDROP0; eauto. rewrite <- DEFSEQ; ss. }
+  - eq_closure_tac. ss. (* TODO: debug this *)
+    rewrite PUBLIC. rewrite PUBS. rewrite PUBLIC0. ss.
+Qed.
+
+Lemma sim_skenv_func_bisim: forall
+          skenv_src skenv_tgt
+          (SIMSKENV: sim_skenv skenv_src skenv_tgt)
+        ,
+          <<DEF: SimSymb.skenv_func_bisim eq skenv_src skenv_tgt>>
+.
+Proof.
+  i.
+  inv SIMSKENV.
+  econs; eauto.
+  - ii. ss.
+    assert(fptr_src = fptr_tgt).
+    { ss. }
+    clarify. unfold Genv.find_funct, Genv.find_funct_ptr in *. des_ifs_safe.
+    erewrite <- DEFS; eauto. des_ifs. esplits; eauto.
+    admit "just use eq".
+  - ii.
+    assert(fptr_src = fptr_tgt).
+    { ss. }
+    clarify. unfold Genv.find_funct, Genv.find_funct_ptr in *. des_ifs_safe.
+    erewrite DEFS; eauto. des_ifs. esplits; eauto.
+    admit "just use eq".
+Qed.
+
